sed -i 's/state_t/treesync_state'

fstar/MLS.TreeSync.API.Types.fst
@@ -5,11 +5,11 @@ open MLS.TreeSync.NetworkTypes
 open MLS.TreeSync.Level0.Types
 
 (** TreeSync state and accessors *)
-type state_t (bytes:Type0) {|bytes_like bytes|} (tkt:treekem_types bytes) = {
+type treesync_state (bytes:Type0) {|bytes_like bytes|} (tkt:treekem_types bytes) = {
   group_id: bytes;
   levels: nat;
   tree: treesync bytes tkt levels 0;
   version: nat;
 }
 
-type index_t (#bytes:Type0) {|bytes_like bytes|} (#tkt:treekem_types bytes) (st:state_t bytes tkt) = i:nat{i < pow2 st.levels}
+type treesync_index (#bytes:Type0) {|bytes_like bytes|} (#tkt:treekem_types bytes) (st:treesync_state bytes tkt) = i:nat{i < pow2 st.levels}
